theories/region_invariants.v
@@ -15,7 +15,39 @@ Class heapG Σ := HeapG {
   heapG_saved_pred :> savedPredG Σ (((STS_states * STS_rels) * (STS_states * STS_rels)) * Word);
   heapG_rel :> inG Σ (authR relUR);
   γrel : gname
-}.
+                   }.
+
+(* We will first define the standard STS for the shared part of the heap *)
+Inductive region_type :=
+| Temporary
+| Permanent
+| Revoked.
+
+Global Instance region_type_EqDecision : EqDecision region_type.
+Proof.
+  intros ρ1 ρ2.
+  destruct ρ1,ρ2;
+    [by left|by right|by right|by right|
+       by left|by right|by right|by right|by left]. 
+Qed.
+Global Instance region_type_finite : finite.Finite region_type.
+Proof.
+  refine {| finite.enum := [Temporary; Permanent; Revoked] ;
+            finite.NoDup_enum := _ ;
+            finite.elem_of_enum := _ |}.
+  - repeat (apply NoDup_cons; split; [repeat (apply not_elem_of_cons;split;auto); apply not_elem_of_nil|]).
+      by apply NoDup_nil.
+  - intros ρ.
+    destruct ρ;apply elem_of_cons;[by left|right|right];
+      apply elem_of_cons;[by left|right];
+        apply elem_of_cons; by left. 
+Qed.           
+Global Instance region_type_countable : Countable region_type.
+Proof. apply finite.finite_countable. Qed. 
+
+Definition std_rel_pub := λ a b, (a = Revoked ∧ b = Temporary).
+Definition std_rel_priv := λ a b, a = Temporary ∨ b = Permanent.
+Global Instance sts_std : STS_STD region_type := {| Rpub := std_rel_pub; Rpriv := std_rel_priv |}.
 
 Section heap.
   Context `{heapG Σ, memG Σ, regG Σ, STSG Σ,
@@ -56,38 +88,6 @@ Section heap.
     | RWLX | RWL => true
     | _ => false
     end.
-
-  (* We will first define the standard STS for the shared part of the heap *)
-  Inductive region_type :=
-  | Temporary
-  | Permanent
-  | Revoked.
-
-  Global Instance region_type_EqDecision : EqDecision region_type.
-  Proof.
-    intros ρ1 ρ2.
-    destruct ρ1,ρ2;
-      [by left|by right|by right|by right|
-         by left|by right|by right|by right|by left]. 
-  Qed.
-  Global Instance region_type_finite : finite.Finite region_type.
-  Proof.
-    refine {| finite.enum := [Temporary; Permanent; Revoked] ;
-              finite.NoDup_enum := _ ;
-              finite.elem_of_enum := _ |}.
-    - repeat (apply NoDup_cons; split; [repeat (apply not_elem_of_cons;split;auto); apply not_elem_of_nil|]).
-        by apply NoDup_nil.
-    - intros ρ.
-      destruct ρ;apply elem_of_cons;[by left|right|right];
-        apply elem_of_cons;[by left|right];
-          apply elem_of_cons; by left. 
-  Qed.           
-  Global Instance region_type_countable : Countable region_type.
-  Proof. apply finite.finite_countable. Qed. 
-
-  Definition std_rel_pub := λ a b, (a = Revoked ∧ b = Temporary).
-  Definition std_rel_priv := λ a b, a = Temporary ∨ b = Permanent.
-  Global Instance sts_std : STS_STD region_type := {| Rpub := std_rel_pub; Rpriv := std_rel_priv |}.
 
   (* Some practical shorthands for projections *)
   Definition std W := W.1.
